\documentclass[aspectratio=169]{beamer}
\usepackage{wallpaper}

% Proof that the Y-Combinator is a fixed point combinator (fix f = (f.fix) f)

\begin{document}
\begin{wallpaperframe}
\[
\text{fix}\, f = f\,(\text{fix}\, f)
\]
\begin{align*}
    Y &= \lambda f.\: (\lambda x.\:f\,(x\,x))\:(\lambda x.\:f\,(x\,x))\, \\
    \Rightarrow Y\, g &= \lambda f.\: (\lambda x.\:f\,(x\,x))\:(\lambda x.\:f\,(x\,x))\, g \\
    &= (\lambda x.\: g\, (x\,x))\:(\lambda x.\: g\, (x\,x)) \\
    &= g\, ((\lambda x.\: g\, (x\,x))\:(\lambda x.\: g\, (x\,x))) \\
    &= g\,(Y\:g)
  \end{align*}

\end{wallpaperframe}
\end{document}